soundness

src/arithmetic.lean
@@ -1,6 +1,6 @@
 import deduction
 
-open language
+namespace fopl
 
 inductive langf : ℕ → Type
 | zero : langf 0
@@ -13,23 +13,43 @@ inductive langp : ℕ → Type
 
 def AL : language := ⟨langf, langp⟩
 
-notation `Ż` := AL.symbolf₀ langf.zero
+def symbol.zero : term AL := vecterm.app langf.zero vecterm.nil
 
-prefix `Ṡ `:max := AL.symbolf₁ langf.succ
+notation `Ż` := symbol.zero
 
-infixl ` +̇ `:92 := AL.symbolf₂ langf.add
+def symbol.succ : term AL → term AL := λ x, vecterm.app langf.succ x
 
-infixl ` ×̇ `:94 := AL.symbolf₂ langf.mult
+prefix `Ṡ `:max := symbol.succ
 
-infixl ` ≤̇ `:90 := (AL.symbolp₂ langp.le)
+def symbol.add : term AL → term AL → term AL := λ x y, vecterm.app langf.add (vecterm.cons x y)
 
-def numeral : ℕ → AL.term
+infixl ` +̇ `:92 := symbol.add 
+
+def symbol.mult : term AL → term AL → term AL := λ x y, vecterm.app langf.mult (vecterm.cons x y)
+
+infixl ` ×̇ `:94 := symbol.mult
+
+def symbol.le : term AL → term AL → form AL := λ x y, form.app langp.le (vecterm.cons x y)
+
+infixl ` ≤̇ `:90 := symbol.le
+
+def numeral : ℕ → term AL
 | 0     := Ż
 | (n+1) := Ṡ (numeral n)
 
-local prefix `˙`:max := numeral
+local notation n`˙`:max := numeral n
 
-inductive robinson : AL.theory
+def bounded_fal (t : term AL) (p : form AL) : form AL := Ȧ(#0 ≤̇ t.sf →̇ p)
+
+notation `[Ȧ`` ≤ `t`]`p := bounded_fal t p
+
+def bounded_ext (t : term AL) (p : form AL) := Ė(#0 ≤̇ t.sf ⩑ p)
+
+notation `[Ė`` ≤ `t`]`p := bounded_ext t p
+
+#check [Ė ≤ #2][Ȧ ≤ #3]Ė[Ȧ ≤ #3](#1 ≤̇ #2)
+
+inductive robinson : theory AL
 | q1 : robinson Ȧ(Ż ≠̇ Ṡ #0)
 | q2 : robinson ȦȦ(Ṡ #0 =̇ Ṡ #1 →̇ #0 =̇ #1)
 | q3 : robinson Ȧ(#0 ≠̇ Ż →̇ Ė(#1 =̇ Ṡ #0))
@@ -41,9 +61,28 @@ inductive robinson : AL.theory
 
 notation `𝐐` := robinson
   
-inductive peano : AL.theory
+inductive peano : theory AL
 | q   : ∀ {p}, 𝐐 p → peano p
-| ind : ∀ (p : AL.form), peano (pˢ(Ż) →̇ Ȧ(p →̇ pᵉ(Ṡ #0)) →̇ Ȧ p)
+| ind : ∀ (p : form AL), peano (p.(Ż) →̇ Ȧ(p →̇ (p.ᵉ(Ṡ #0))) →̇ Ȧ p)
 
 notation `𝐏𝐀` := peano
 
+inductive bounded_peano (C : set (form AL)) : theory AL
+| q   : ∀ {p}, 𝐐 p → bounded_peano p
+| ind : ∀ {p : form AL}, p ∈ C → bounded_peano (p.(Ż) →̇ Ȧ(p →̇ (p.ᵉ(Ṡ #0))) →̇ Ȧ p)
+
+mutual inductive sigma, pie
+with sigma : ℕ → form AL → Prop
+| op : ∀ {p : form AL}, p.op → sigma 0 p
+| bd_fal : ∀ {p} {n t}, sigma n p → sigma n [Ȧ ≤ t]p
+| bd_ext : ∀ {p} {n t}, sigma n p → sigma n [Ė ≤ t]p
+| qt : ∀ {p} {n}, pie n p → sigma (n+1) Ėp 
+with pie : ℕ → form AL → Prop
+| op : ∀ {p : form AL}, p.op → pie 0 p
+| bd_fal : ∀ {p} {n t}, pie n p → pie n [Ȧ ≤ t]p
+| bd_ext : ∀ {p} {n t}, pie n p → pie n [Ė ≤ t]p
+| qt : ∀ {p} {n}, sigma n p → pie (n+1) Ȧp 
+
+
+
+end fopl
