src/deduction.lean
@@ -2,81 +2,84 @@ import fopl
 
 universe u
 
-namespace language
+namespace fopl
 variables {L : language.{u}}
 
-def theory (L : language) := L.form → Prop
+def theory (L : language) := form L → Prop
 
-inductive theory.sf (T : L.theory) : L.theory
-| intro : ∀ {p : L.form}, T p → theory.sf p.sf
+inductive theory.sf (T : theory L) : theory L
+| intro : ∀ {p : form L}, T p → theory.sf p.sf
 
 prefix `⇑`:max := theory.sf
 
-inductive provable : L.theory → L.form → Prop
-| gen : ∀ {T : theory L} {p}, provable (⇑T) p → provable T (Ȧp)
-| mp  : ∀ {T : theory L} {p q}, provable T (p →̇ q) → provable T p → provable T q
-| ax  : ∀ {T : theory L} {p}, T p → provable T p
-| p1  : ∀ (T : theory L) (p q), provable T (p →̇ q →̇ p)
-| p2  : ∀ (T : theory L) (p q r), provable T ((p →̇ q →̇ r) →̇ (p →̇ q) →̇ p →̇ r)
-| p3  : ∀ (T : theory L) (p q), provable T ((¬̇ p →̇ ¬̇ q) →̇ q →̇ p)
-| q1  : ∀ (T : theory L) (p t), provable T (Ȧ p →̇ p.(t))
-| q2  : ∀ (T : theory L) (p q), provable T (Ȧ (p →̇ q) →̇ Ȧ p →̇ Ȧ q)
-| q3  : ∀ (T : theory L) (p), provable T (p →̇ Ȧ p.sf)
-| e1  : ∀ (T : theory L) (t), provable T (t =̇ t)
-| e2  : ∀ (T : theory L) (p : L.form) (t u), provable T (t =̇ u →̇ p.(t) →̇ p.(u))
+inductive provable : theory L → form L → Prop
+| GE : ∀ {T : theory L} {p}, provable ⇑T p → provable T (Ȧp)
+| MP : ∀ {T : theory L} {p q}, provable T (p →̇ q) → provable T p → provable T q
+| AX : ∀ {T : theory L} {p}, T p → provable T p
+| p1 : ∀ (T : theory L) (p q), provable T (p →̇ q →̇ p)
+| p2 : ∀ (T : theory L) (p q r), provable T ((p →̇ q →̇ r) →̇ (p →̇ q) →̇ p →̇ r)
+| p3 : ∀ (T : theory L) (p q), provable T ((¬̇ p →̇ ¬̇ q) →̇ q →̇ p)
+| q1 : ∀ (T : theory L) (p t), provable T (Ȧ p →̇ p.(t))
+| q2 : ∀ (T : theory L) (p q), provable T (Ȧ (p →̇ q) →̇ Ȧ p →̇ Ȧ q)
+| q3 : ∀ (T : theory L) (p), provable T (p →̇ Ȧ p.sf)
+| e1 : ∀ (T : theory L) (t), provable T (t =̇ t)
+| e2 : ∀ (T : theory L) (p : form L) (t u), provable T (t =̇ u →̇ p.(t) →̇ p.(u))
 
 infix ` ⊢̇ `:60 := provable
 
 attribute [simp] provable.p1 provable.p2 provable.p3 provable.q1 provable.q2 provable.q3
   provable.e1 provable.e2
 
-def theory.consistent (T : L.theory) : Prop := ¬∃p, (T ⊢̇ p) ∧ (T ⊢̇ ¬̇p) 
+def theory.consistent (T : theory L) : Prop := ¬∃p, (T ⊢̇ p) ∧ (T ⊢̇ ¬̇p) 
 
-inductive theory.add (T : L.theory) (p : L.form) : L.theory 
+inductive theory.add (T : theory L) (p : form L) : theory L 
 | new : theory.add p
 | old : ∀ {q}, T q → theory.add q
 
 infixl ` ¦ `:60 := theory.add
 
-def theory.delete (T : L.theory) (p : L.form) : L.theory := λ q, T q ∧ q ≠ p
+def theory.delete (T : theory L) (p : form L) : theory L := λ q, T q ∧ q ≠ p
 
-def theory.include (T U : L.theory) : Prop := ∀ p, T p → U p
+def theory.include (T U : theory L) : Prop := ∀ p, T p → U p
 
-instance : has_subset L.theory := ⟨theory.include⟩
+instance : has_subset (theory L) := ⟨theory.include⟩
 
 namespace provable
-variables (T : L.theory)
+variables (T : theory L)
 
 @[simp] lemma pp (p) : T ⊢̇ p →̇ p :=
 begin
   have l₀ : T ⊢̇ (p →̇ (p →̇ p) →̇ p) →̇ (p →̇ p →̇ p) →̇ p →̇ p, simp,
   have l₁ : T ⊢̇ p →̇ (p →̇ p) →̇ p, simp,
-  have l₂ : T ⊢̇ (p →̇ p →̇ p) →̇ p →̇ p, refine l₀.mp l₁,
+  have l₂ : T ⊢̇ (p →̇ p →̇ p) →̇ p →̇ p, refine l₀.MP l₁,
   have l₃ : T ⊢̇ p →̇ p →̇ p, simp,
-  refine l₂.mp l₃
+  refine l₂.MP l₃
 end
+
+@[simp] lemma add (p) : T ¦ p ⊢̇ p :=
+AX (theory.add.new)
 
 variables {T}
 
 @[simp] lemma imp_r {p} (h : T ⊢̇ p) (q) : T ⊢̇ q →̇ p :=
 by { have : T ⊢̇ p →̇ q →̇ p, simp,
-     exact this.mp h }
+     exact this.MP h }
 
 lemma imp_trans {p q r} : (T ⊢̇ p →̇ q) → (T ⊢̇ q →̇ r) → (T ⊢̇ p →̇ r) := λ h₁ h₂,
 begin
   have l₁ : T ⊢̇ (p →̇ q →̇ r) →̇ (p →̇ q) →̇ (p →̇ r), simp,  
   have l₂ : T ⊢̇ (p →̇ q →̇ r), simp[h₂],
-  have l₃ : T ⊢̇ (p →̇ q) →̇ (p →̇ r), from l₁.mp l₂,
-  exact l₃.mp h₁
+  have l₃ : T ⊢̇ (p →̇ q) →̇ (p →̇ r), from l₁.MP l₂,
+  exact l₃.MP h₁
 end
 
 lemma inclusion {p} (h : T ⊢̇ p) : ∀ {U}, T ⊆ U → U ⊢̇ p :=
 begin
   induction h with T p hyp_p IH T p q hyp_pq hyp_p IH₁ IH₂ T p hyp_p; try { simp },
-  { intros U hyp, refine gen (IH (λ x h, _)), cases h with p hp,
+  { intros U hyp, refine GE (IH (λ x h, _)), cases h with p hp,
     refine theory.sf.intro _, exact hyp _ hp },
-  { intros U hyp, exact (IH₁ hyp).mp (IH₂ hyp) },
-  { intros U hyp, exact ax (hyp _ hyp_p) }
+  { intros U hyp, exact (IH₁ hyp).MP (IH₂ hyp) },
+  { intros U hyp, exact AX (hyp _ hyp_p) }
 end
 
 @[simp] lemma weakening {q} (h : T ⊢̇ q) (p) : T ¦ p ⊢̇ q :=
@@ -91,27 +94,145 @@ begin
     have lmm₂ : T.delete q ⊢̇ Ȧ q.sf →̇ Ȧ p,
     { suffices : T.delete q ⊢̇ Ȧ(q.sf →̇ p),
       { have lmm : T.delete q ⊢̇ Ȧ(q.sf →̇ p) →̇ Ȧ q.sf →̇ Ȧ p, simp,
-        exact lmm.mp this },
-      refine gen (inclusion IH (λ x h, _)), 
+        exact lmm.MP this },
+      refine GE (inclusion IH (λ x h, _)), 
       rcases h with ⟨h, neq⟩, rcases h with ⟨p', h'⟩,
       refine theory.sf.intro ⟨h', λ c, _⟩,
       rw c at neq, exact neq rfl },
     exact lmm₁.imp_trans lmm₂ },
   { have : T.delete q ⊢̇ (q →̇ p₁ →̇ p₂) →̇ (q →̇ p₁) →̇ (q →̇ p₂), simp, 
-    have : T.delete q ⊢̇ (q →̇ p₁) →̇ q →̇ p₂, from this.mp (IH₁ _),
-    exact this.mp (IH₂ _) },
+    have : T.delete q ⊢̇ (q →̇ p₁) →̇ q →̇ p₂, from this.MP (IH₁ _),
+    exact this.MP (IH₂ _) },
   { by_cases eqn : p = q,
     { simp[eqn] },
-    { have : T.delete q ⊢̇ p, from ax ⟨hyp_p, eqn⟩,
+    { have : T.delete q ⊢̇ p, from AX ⟨hyp_p, eqn⟩,
       simp[this] } }
 end
 
-theorem deduction {p q} : (T ¦ p ⊢̇ q) → (T ⊢̇ p →̇ q) := λ h,
-by { have : (T ¦ p).delete p ⊢̇ p →̇ q, from delete_imply h p,
-     refine inclusion this (λ x h, _), rcases h with ⟨h, neq⟩,
-     cases h; simp* at* }
+theorem deduction {p q} : (T ¦ p ⊢̇ q) ↔ (T ⊢̇ p →̇ q) :=
+⟨λ h, by { have : (T ¦ p).delete p ⊢̇ p →̇ q, from delete_imply h p,
+           refine inclusion this (λ x h, _), rcases h with ⟨h, neq⟩,
+           cases h; simp* at* },
+ λ h, by { have : T ¦ p ⊢̇ p →̇ q, from weakening h p,
+           exact this.MP (by simp) }⟩ 
 
+@[simp] lemma dne (p) : T ⊢̇ ¬̇¬̇p →̇ p :=
+begin
+  have llm₁ : T ¦ ¬̇¬̇p ⊢̇ ¬̇¬̇p, simp,   
+  have llm₂ : T ¦ ¬̇¬̇p ⊢̇ ¬̇¬̇p →̇ ¬̇¬̇¬̇¬̇p →̇ ¬̇¬̇p, simp,
+  have llm₃ : T ¦ ¬̇¬̇p ⊢̇ ¬̇¬̇¬̇¬̇p →̇ ¬̇¬̇p, from llm₂.MP llm₁,
+  have llm₄ : T ¦ ¬̇¬̇p ⊢̇ (¬̇¬̇¬̇¬̇p →̇ ¬̇¬̇p) →̇ ¬̇p →̇ ¬̇¬̇¬̇p, simp,
+  have llm₅ : T ¦ ¬̇¬̇p ⊢̇ ¬̇p →̇ ¬̇¬̇¬̇p, from llm₄.MP llm₃,
+  have llm₆ : T ¦ ¬̇¬̇p ⊢̇ (¬̇p →̇ ¬̇¬̇¬̇p) →̇ ¬̇¬̇p →̇ p, simp,
+  have llm₇ : T ¦ ¬̇¬̇p ⊢̇ ¬̇¬̇p →̇ p, from llm₆.MP llm₅,
+  have llm₈ : T ¦ ¬̇¬̇p ⊢̇ p, from llm₇.MP llm₁,
+  exact deduction.mp llm₈  
+end
+
+@[simp] lemma dni (p) : T ⊢̇ p →̇ ¬̇¬̇p :=
+by { have : T ⊢̇ (¬̇¬̇¬̇p →̇ ¬̇p) →̇ p →̇ ¬̇¬̇p, simp,
+     exact this.MP (by simp) }
+
+lemma dn_iff {p} : T ⊢̇ ¬̇¬̇p ↔ T ⊢̇ p :=
+⟨λ h, (show T ⊢̇ ¬̇¬̇p →̇ p, by simp).MP h, λ h,(show T ⊢̇ p →̇ ¬̇¬̇p, by simp).MP h⟩
+
+lemma explosion {p} (h₁ : T ⊢̇ p) (h₂ : T ⊢̇ ¬̇p) {q} : T ⊢̇ q :=
+begin
+  have : T ⊢̇ ¬̇p →̇ ¬̇q →̇ ¬̇p, simp,
+  have : T ⊢̇ ¬̇q →̇ ¬̇p, from this.MP h₂,
+  have : T ⊢̇ p →̇ q, from (show T ⊢̇ (¬̇q →̇ ¬̇p) →̇ p →̇ q, by simp).MP this,
+  exact this.MP h₁
+end
+
+lemma contra {p q} : (T ⊢̇ ¬̇p →̇ ¬̇q) ↔ (T ⊢̇ q →̇ p) :=
+⟨λ h, (show T ⊢̇ (¬̇p →̇ ¬̇q) →̇ q →̇ p, by simp).MP h, λ h,
+  by { refine (show T ⊢̇ (¬̇¬̇q →̇ ¬̇¬̇p) →̇ ¬̇p →̇ ¬̇q, by simp).MP _,
+       have : T ⊢̇ ¬̇¬̇q →̇ p, from (show T ⊢̇ ¬̇¬̇q →̇ q, by simp).imp_trans h,
+       exact this.imp_trans (show T ⊢̇ p →̇ ¬̇¬̇p, by simp) }⟩
+
+lemma neg_hyp {p} (h : T ⊢̇ p →̇ ¬̇p) : T ⊢̇ ¬̇p :=
+begin
+  have : T ¦ p ⊢̇ ¬̇(p →̇ ¬̇p),
+  { have lmm₁ : T ¦ p ⊢̇ p, simp,
+    have lmm₂ : T ¦ p ⊢̇ ¬̇p, from (weakening h _).MP lmm₁,
+    exact explosion lmm₁ lmm₂ },
+  have : T ⊢̇ p →̇ ¬̇(p →̇ ¬̇p), from deduction.mp this,
+  have : T ⊢̇ (p →̇ ¬̇p) →̇ ¬̇p, from (dni _).imp_trans (contra.mpr this),
+  exact this.MP h
+end
+
+lemma raa {p} (q) (h₁ : T ¦ p ⊢̇ q) (h₂ : T ¦ p ⊢̇ ¬̇q) : T ⊢̇ ¬̇p :=
+neg_hyp (deduction.mp (explosion h₁ h₂))
+
+@[simp] lemma and {p q} : (T ⊢̇ p ⩑ q) ↔ (T ⊢̇ p ∧ T ⊢̇ q) :=
+⟨λ h, by { simp[form.and] at h, split,
+   { have : T ¦ ¬̇p ¦ p ⊢̇ ¬̇q, 
+     from explosion (show T ¦ ¬̇p ¦ p ⊢̇ p, by simp) (show T ¦ ¬̇p ¦ p ⊢̇ ¬̇p, by simp),
+     have : T ⊢̇ ¬̇p →̇ p →̇ ¬̇q, from (deduction.mp (deduction.mp this)),
+     have : T ⊢̇ ¬̇(p →̇ ¬̇q) →̇ p := (contra.mpr this).imp_trans (by simp),
+     exact this.MP h },
+   { have : T ⊢̇ ¬̇q →̇ p →̇ ¬̇q, simp,
+     have : T ⊢̇ ¬̇(p →̇ ¬̇q) →̇ q, from (contra.mpr this).imp_trans (by simp),
+     exact this.MP h } },
+ λ h, by {simp[form.and], rcases h with ⟨h₁, h₂⟩,
+   show T ⊢̇ ¬̇(p →̇ ¬̇q),
+   have : T ¦ p →̇ ¬̇q ⊢̇ ¬̇q, from (add _ _).MP (by simp[h₁]),
+   have : T ⊢̇ (p →̇ ¬̇q) →̇ ¬̇q, from deduction.mp this,
+   have : T ⊢̇ q →̇ ¬̇(p →̇ ¬̇q), from (dni _).imp_trans (contra.mpr this),
+   exact this.MP h₂ }⟩
+
+lemma iff {p q} : (T ⊢̇ p ↔̇ q) ↔ (T ⊢̇ p →̇ q ∧ T ⊢̇ q →̇ p) :=
+by simp[form.iff]
+
+lemma subst₁ {p} (h : T ⊢̇ Ȧp) (t) : T ⊢̇ p.(t) :=
+(show T ⊢̇ Ȧp →̇ p.(t), by simp).MP h
+
+lemma subst₂ {p} (h : T ⊢̇ ȦȦp) (t u) : T ⊢̇ p.(t, u) :=
+begin
+  have : p.(t, u) = (p.rew (#0 ^ˢ u.sf ^ᵉ idvar)).(t),
+  { simp [form.subst₂, form.subst₁, form.nested_rew],
+    congr, funext n,
+    cases n; simp[slide, vecterm.rew],
+    cases n; simp[slide, embed, vecterm.rew] },
+  sorry
+end
+
+@[simp] lemma sf_dsb {p : form L} : ⇑T ¦ p.sf = ⇑(T ¦ p) :=
+begin
+  ext x, split; intros h,
+  { cases h with h hx, refine theory.sf.intro theory.add.new,
+    cases hx with p hp, refine theory.sf.intro (theory.add.old hp) },
+  { cases h with q hq, cases hq with _ hq, refine theory.add.new,
+    refine theory.add.old (theory.sf.intro hq) }
+end
+
+lemma use {p : form L} (t) (h : T ⊢̇ p.(t)) : T ⊢̇ Ėp :=
+begin
+  simp[form.ex],
+  refine raa (p.(t)) (by simp[h]) (deduction.mpr _),
+  have : ¬̇p.(t) = (¬̇p).(t) := rfl,
+  simp[this],
+end
+
+lemma eq_symm : ∀ {t u}, (T ⊢̇ t =̇ u) ↔ (T ⊢̇ u =̇ t) :=
+begin
+  suffices : ∀ t u, (T ⊢̇ t =̇ u) → (T ⊢̇ u =̇ t),
+  { intros t u, refine ⟨this _ _, this _ _⟩ },
+  intros t u h,
+  have : ∀ v, v =̇ t = (#0 =̇ t.sf).(v),
+  { intros v, simp[form.subst₁, form.rew, vecterm.rew, slide] },
+  have : T ⊢̇ t =̇ u →̇ t =̇ t →̇ u =̇ t, { rw [this t, this u], simp },
+  exact (this.MP h).MP (by simp)
+end
+
+lemma eq_trans {t₁ t₂ t₃} : (T ⊢̇ t₁ =̇ t₂) → (T ⊢̇ t₂ =̇ t₃) → (T ⊢̇ t₁ =̇ t₃) := λ h₁ h₂,
+begin
+  have : ∀ u v : term L, u =̇ v = (u.sf =̇ #0).(v),
+  { intros v, simp[form.subst₁, form.rew, vecterm.rew, slide] },
+  have : T ⊢̇ t₂ =̇ t₃ →̇ t₁ =̇ t₂ →̇ t₁ =̇ t₃, { rw [this t₁ t₂, this t₁ t₃], simp },
+  exact (this.MP h₂).MP h₁
+end
 
 end provable
 
-end language
+end fopl
