src/lib.lean
@@ -1,0 +1,27 @@
+import tactic
+
+universe u
+
+inductive dvector (α : Type u) : ℕ → Type u
+| nil {} : dvector 0
+| cons   : ∀ {n}, α → dvector n → dvector (n+1)
+
+notation a :: b  := dvector.cons a b
+
+namespace dvector
+variables {α : Type u}
+
+@[simp] def unary (a : α) : dvector α 1 := a :: nil
+
+@[simp] def extract : dvector α 1 → α
+| (a :: nil) := a
+
+@[simp] lemma extract_nil : ∀ (v : dvector α 1), v.extract :: nil = v
+| (a :: nil) := rfl
+
+@[simp] protected def append : ∀ {n}, dvector α n → ∀ {m}, dvector α m → dvector α (m + n)
+| _ nil      _ l := l
+| _ (a :: l) _ k := a :: (append l k)
+
+
+end dvector
