src/semantics.lean
@@ -1,0 +1,102 @@
+import deduction
+
+universes u v
+
+namespace fopl
+open dvector
+
+structure model (L : language.{u}) :=
+(dom : Type v)
+(fn : ∀ {n}, L.fn n → dvector dom n → dom)
+(pr : ∀ {n}, L.pr n → dvector dom n → Prop)
+
+variables {L : language.{u}} {M : model L}
+
+def vecterm.val (e : ℕ → M.dom) : ∀ {n} (t : vecterm L n), dvector M.dom n
+| _ vecterm.nil        := nil
+| _ (vecterm.cons a v) := a.val.append v.val
+| _ (#x)               := unary (e x)
+| _ (vecterm.app f v)  := unary (M.fn f v.val)
+
+def term.val (e : ℕ → M.dom) (t : term L) : M.dom := (t.val e).extract
+
+def form.val : (ℕ → M.dom) → form L → Prop
+| e (form.app p v) := M.pr p (v.val e)
+| e (t =̇ u)        := t.val e = u.val e
+| e (p →̇ q)       := p.val e → q.val e
+| e (¬̇p)           := ¬(p.val e)
+| e (Ȧp)           := ∀ d : M.dom, (p.val (d ^ˢ e))
+
+def models (M : model L) (p : form L) : Prop := ∀ (e : ℕ → M.dom), p.val e
+infix ` ⊧ `:50 := models
+
+def modelsth (M : model L) (T : form L → Prop) : Prop := ∀ (e : ℕ → M.dom) p, T p → p.val e
+infix ` ⊧ₜₕ `:50 := modelsth
+
+lemma rew_val_eq : ∀ (s : ℕ → term L) {n} (t : vecterm L n) (e : ℕ → M.dom),
+  (t.rew s).val e = t.val (λ n, (s n).val e)
+| _ _ vecterm.nil        _ := rfl
+| _ _ (vecterm.cons a v) _ := by simp[vecterm.val, vecterm.rew, rew_val_eq _ a, rew_val_eq _ v]
+| _ _ (#x)               _ := by simp[vecterm.val, vecterm.rew, term.val]
+| _ _ (vecterm.app f v)  _ := by simp[vecterm.val, vecterm.rew, rew_val_eq _ v]
+
+@[simp] lemma sf_slide_val {n} (t : vecterm L n) : ∀ (e : ℕ → M.dom) d, t.sf.val (d ^ˢ e) = t.val e :=
+by induction t; simp[vecterm.val, slide]; simp*
+
+lemma rew_val_iff : ∀ (s : ℕ → term L) (p : form L) (e : ℕ → M.dom),
+  (p.rew s).val e ↔ p.val (λ n, (s n).val e)
+| _ (form.app p v) _ := by simp[form.val, form.rew, rew_val_eq]
+| _ (t =̇ u)        _ := by simp[form.val, form.rew, term.val, rew_val_eq]
+| _ (p →̇ q)       _ := by simp[form.val, form.rew, rew_val_iff _ p, rew_val_iff _ q]
+| _ (¬̇p)           _ := by simp[form.val, form.rew, rew_val_iff _ p]
+| s (Ȧp)           e := by { simp[form.val, form.rew, rew_val_iff _ p], refine forall_congr (λ d, _),
+    have : (λ n, ((#0 ^ˢ λ x, (s x).sf) n : term L).val (d ^ˢ e)) = (d ^ˢ λ n, (s n).val e),
+    { funext n,cases n; simp[slide, term.val, vecterm.val] },
+    simp[this] }
+
+@[simp] lemma sf_slide_val_iff : ∀ (p : form L) (e : ℕ → M.dom) d, p.sf.val (d ^ˢ e) = p.val e
+| (form.app p v) _ _ := by simp[form.val]
+| (t =̇ u)        _ _ := by simp[form.val, term.val]
+| (p →̇ q)       _ _ := by simp[form.val, sf_slide_val_iff p, sf_slide_val_iff q]
+| (¬̇p)           _ _ := by simp[form.val, sf_slide_val_iff p]
+| (Ȧp)           e d := by simp[form.val, term.val, vecterm.val, form.sf, rew_val_iff, slide]
+
+private lemma modelsth_sf {T} : M ⊧ₜₕ T → M ⊧ₜₕ ⇑T := λ h e p hyp_p,
+by { cases hyp_p with p hyp_p', simp[rew_val_iff],
+     refine h _ _ hyp_p' }
+
+theorem soundness {T : theory L} : ∀ {p}, T ⊢̇ p → ∀ {M}, M ⊧ₜₕ T → M ⊧ p := λ p hyp,
+begin
+  induction hyp,
+  case fopl.provable.GE : T p hyp_p IH
+  { intros M hyp_T e d, exact IH (modelsth_sf hyp_T) _ },
+  case fopl.provable.MP : T p q hyp_pq hyp_p IH_pq IH_p
+  { intros M hyp_T e, exact IH_pq hyp_T e (IH_p hyp_T e) },
+  case fopl.provable.AX : T p hyp_p
+  { intros M hyp_T e, exact hyp_T e _ hyp_p },
+  case fopl.provable.p1 : T p q
+  { intros M hyp_T e h₁ h₂, exact h₁ },
+  case fopl.provable.p2 : T p q r
+  { intros M hyp_T e h₁ h₂ h₃, exact (h₁ h₃) (h₂ h₃) },
+  case fopl.provable.p3 : T p q
+  { intros M hyp_T e h₁, simp[form.val], contrapose, exact h₁ },
+  case fopl.provable.q1 : T p t
+  { intros M hyp_T e h, simp[form.val, form.subst₁, rew_val_iff] at h ⊢,
+    have : (λ n, ((t ^ˢ vecterm.var) n).val e) = (t.val e) ^ˢ e,
+    { funext n, cases n; simp[slide, term.val, vecterm.val] },
+    rw this, exact h _ },
+  case fopl.provable.q2 : T p q
+  { intros M hyp_T e h₁ h₂ d, exact (h₁ d) (h₂ d) },
+  case fopl.provable.q3 : T p
+  { intros M hyp_T e h d, simp, exact h },
+  case fopl.provable.e1 : T t
+  { intros M hyp_T e, simp[form.val] },
+  case fopl.provable.e2 : T p t u
+  { intros M hyp_T e, simp[form.val, form.subst₁, rew_val_iff],
+    intros eqn h,
+    have : (λ n, ((u ^ˢ vecterm.var) n).val e) = (λ n, ((t ^ˢ vecterm.var) n).val e),
+    { funext n, cases n; simp[slide, term.val, eqn] },
+    simp[this, h] }
+end
+
+end fopl
